%\section{Appendix}
\begin{appendix}
\appendixpage
\chapter{}
\renewcommand{\thechapter}{\Roman{chapter}}

\pagestyle{empty}
\section{\label{apen:derivationdegenerate}Fredholm IE of Second Kind and Analytical Solution for Degenerate Kernel}
\label{appendix-1}
Here we discuss derivation of analytical solution of non-homogeneous Fredholm integral equation of second kind.


The Fredholm integral equation of second kind

\begin{equation}
\phi(x)=f(x)+\lambda\int_a^b K(x,y)\phi(y)dy
\end{equation}
with a {\em degenerate kernel} 
\begin{equation}
 K(x,y) = \sum\limits_{i=1}^na_i(x)b_i(y)
\end{equation}
defined over domain of $x,y \in [a,b]$ can be expanded, by substituting kernel into integral equation as
\begin{equation}
 \phi(x)=f(x)+\lambda\int_a^b \sum\limits_{i=1}^na_i(x)b_i(y)\phi(y)dy
\end{equation}
above equation can be rewritten, by changing the order of integration ans summation, in the form
\begin{equation}\label{eq:orderchange}
 \phi(x)=f(x)+\lambda \sum\limits_{i=1}^na_i(x)\int_a^b b_i(y)\phi(y)dy
\end{equation}
let unknown constants $ c_i, i=0, 1, ..., n $ be defined as
\begin{equation}
 c_i=\int_a^b b_i(y)\phi(y)dy
\end{equation}
thus Equation \ref{eq:orderchange}, after substituting $c_i, i=0, 1, ..., n$, becomes
\begin{equation}\label{eq:simplephi}
 \phi(x)=f(x)+\lambda \sum\limits_{i=1}^nc_ia_i(x) 
\end{equation}
Now, problem reduce to the finding unknowns $ c_i, i=0, 1, ..., n $. We substitute Equation \ref{eq:simplephi} into Equation \ref{eq:orderchange} we get,
\begin{equation}
f(x)+\lambda \sum\limits_{i=1}^nc_ia_i(x) =f(x)+\lambda \sum\limits_{i=1}^na_i(x)\int_a^b b_i(y)\quad[f(y)+\lambda \sum\limits_{i=1}^na_i(y) c_idy] \quad
\end{equation}
\begin{equation}
\sum\limits_{i=1}^nc_ia_i(x) -\sum\limits_{i=1}^na_i(x)\int_a^b b_i(y)(f(y)+\lambda \sum\limits_{i=1}^na_i(y) c_idy)=0
\end{equation}
\begin{equation}
\sum\limits_{i=1}^na_i(x)\quad( c_i-\int_a^b b_i(y)\quad[f(y)+\lambda \sum\limits_{i=1}^na_i(y) c_idy])=0
\end{equation}
if chosen $a_i(x), i=0, 1, ..., n $ is linearly independent, then above equation is true if and only if 
\begin{equation}\label{eq:linearsystem}
c_i-\int_a^b b_i(y)\quad[f(y)+\lambda \sum\limits_{i=1}^na_i(y) c_idy]=0,\quad i=0, 1, ..., n 
\end{equation}
let 
\begin{equation}
f_i=\int_a^b b_i(y)f(y),\quad i=0, 1, ..., n 
\end{equation}
and 
\begin{equation}
a_{ij}=\int_a^b b_i(y)a_j(y) dy=0,\quad i,j \in \{0, 1, ..., n\} 
\end{equation}
Now changing summation and integration order, Equation \ref{eq:linearsystem} is rewritten as
\begin{equation}\label{eq:linearsystem}
c_i=f_i+\lambda \sum\limits_{i=1}^na_{ij},\quad i=0, 1, ..., n 
\end{equation}
Finally we get system of linear equation of order n and n unknowns $c_i$. Substituting $c_i$ into Equation \ref{eq:simplephi} we get the solution of the Integral Equation as 
 \begin{equation}\label{eq:simplephi}
 \phi(x)=f(x)+\lambda \sum\limits_{i=1}^nc_ia_i(x) 
\end{equation}

\end{appendix}